streamlined the definitions of igraph and insfrastructure to include the selector functions into the datatype definitions. Adapted the proofs also in CredisScoringLocae because now the names of simplification rules needed to be changed from gra.simps -> ipgraph.sel(1) etc. For infrasrtructure there seemed to be a problem therefore I reintrouduced separate lemma graphI_simps for graphI.simps etc. In addition I now deleted in CreditScoringLocale the old obsolete version of the proof for the application of the PCR cycle that used the AG(EF pci --> EF DO ...) formula instead inlining into AG( pc_i --> EF DO ...)

CreditScoringInfrastructure.thy
@@ -43,19 +43,21 @@ type_synonym data = \<open>location \<times> nat \<times> dob \<times> ethnicity
 type_synonym dlm = \<open>actor \<times> actor set\<close>
 
 datatype igraph = Lgraph 
-                     \<open>(location \<times> location)set\<close>
-                     \<open>location \<Rightarrow> identity set\<close>
-                     \<open> identity \<Rightarrow> dlm \<times> data\<close>
-                     \<open> data \<Rightarrow> bool\<close>
-                     \<open>(identity \<times> bool option)set\<close>
+                    (gra: \<open>(location \<times> location)set\<close>)
+                    (agra: \<open>location \<Rightarrow> identity set\<close>)
+                    (dgra: \<open> identity \<Rightarrow> dlm \<times> data\<close>)
+                    (bb: \<open> data \<Rightarrow> bool\<close>)
+                    (requests: \<open>(identity \<times> bool option)set\<close>)
 
 
 datatype infrastructure = 
-         Infrastructure \<open>igraph\<close> 
+         Infrastructure \<open>igraph\<close>
                         \<open>[igraph, location] \<Rightarrow> policy set\<close>
                        
 primrec loc :: \<open>location \<Rightarrow> nat\<close>
 where  \<open>loc(Location n) = n\<close>
+
+(*
 primrec gra :: \<open>igraph \<Rightarrow> (location * location)set\<close>
 where  \<open>gra(Lgraph g a d b e) = g\<close>
 primrec agra :: \<open>igraph \<Rightarrow> (location \<Rightarrow> identity set)\<close>
@@ -66,6 +68,9 @@ primrec bb :: \<open>igraph \<Rightarrow> (data \<Rightarrow> bool)\<close>
 where  \<open>bb(Lgraph g a d b e) = b\<close>
 primrec requests:: \<open>igraph \<Rightarrow> (identity * bool option)set\<close>
   where \<open>requests(Lgraph g a d b e) = e\<close>
+*)
+lemma agra_simps: \<open>agra (Lgraph g a d b e) = a\<close>
+ by (rule CreditScoringInfrastructure.igraph.sel(2))
 
 definition nodes :: \<open>igraph \<Rightarrow> location set\<close>
 where \<open>nodes g == { x. (? y. ((x,y): gra g) | ((y,x): gra g))}\<close>
@@ -75,11 +80,20 @@ where  "actors_graph g == {x. ? y. y : nodes g \<and> x \<in> (agra g y)}"
 
 text \<open>There are projection functions text{@ \<open>graphI\<close>} and text{@ \<open>delta\<close>} when applied
 to an infrastructure return the graph and the policy, respectively.\<close>
+
+
 primrec graphI :: "infrastructure \<Rightarrow> igraph"
 where "graphI (Infrastructure g d) = g"
 primrec delta :: "[infrastructure, igraph, location] \<Rightarrow> policy set"
 where "delta (Infrastructure g d) = d"
 
+(*
+lemma graphI_simps[simp]: \<open>graphI (Infrastructure g d) = g\<close>
+  by (rule infrastructure.sel(1))
+
+lemma delta_simps[simp]: \<open>delta (Infrastructure g d) = d\<close>
+  by (rule infrastructure.sel(2))
+*)
 text \<open>Predicates and projections for the labels to encode their meaning.\<close>
 definition owner :: "dlm * data \<Rightarrow> actor" where "owner d \<equiv> fst(fst d)"
 definition owns :: "[igraph, location, actor, dlm * data] \<Rightarrow> bool"
